maps as sorted lists (unproven)

bedrock2/src/String.v
@@ -1,2 +1,20 @@
+Require Coq.NArith.BinNatDef.
+
 Require Export Coq.Strings.String.
 Definition eqb a b := andb (String.prefix a b) (String.prefix b a).
+
+Module Ascii.
+  Import Coq.NArith.BinNatDef.
+  Definition eqb (c d : Ascii.ascii) : bool := N.eqb (Ascii.N_of_ascii c) (Ascii.N_of_ascii d).
+  Definition ltb (c d : Ascii.ascii) : bool := N.ltb (Ascii.N_of_ascii c) (Ascii.N_of_ascii d).
+End Ascii.
+
+Fixpoint ltb (a b : string) : bool :=
+  match a, b with
+    | EmptyString, String _ _ => true
+    | String x a', String y b' =>
+      if Ascii.eqb x y
+      then ltb a' b'
+      else Ascii.ltb x y
+    | _, _ => false
+  end.
