bedrock2/src/Map/SortedList.v
@@ -1,0 +1,54 @@
+Local Set Primitive Projections.
+Require Import bedrock2.Macros bedrock2.Map.
+Require Coq.Lists.List.
+
+(* TODO: move me? *)
+Definition minimize_eq_proof{A: Type}(eq_dec: forall (x y: A), {x = y} + {x <> y}){x y: A}    (pf: x = y): x = y :=
+  match eq_dec x y with
+  | left p => p
+  | right n => match n pf: False with end
+  end.
+
+Module Import parameters.
+  Class parameters := {
+    key : Type;
+    value : Type;
+    key_eqb : key -> key -> bool;
+    key_ltb : key -> key -> bool
+  }.
+End parameters. Notation parameters := parameters.parameters.
+
+Section UnorderedList.
+  Context {p : unique! parameters}.
+  Fixpoint put m (k:key) (v:value) : list (key * value) :=
+    match m with
+    | nil => cons (k, v) nil
+    | cons (k', v') m' =>
+      if key_eqb k k'
+      then cons (k, v) m'
+      else 
+        if key_ltb k k'
+        then cons (k, v) m
+        else cons (k', v') (put m' k v)
+    end.
+  Fixpoint sorted (m : list (key * value)) :=
+    match m with
+    | cons (k1, _) ((cons (k2, _) m'') as m') => andb (key_ltb k1 k2) (sorted m')
+    | _ => true
+    end.
+  Record rep := { value : list (key * value) ; ok : sorted value = true }.
+  Lemma sorted_put m k v : sorted m = true -> sorted (put m k v) = true. Admitted.
+  Instance map : map key parameters.value :=
+    let wrapped_put m k v := Build_rep (put (value m) k v) (minimize_eq_proof Bool.bool_dec (sorted_put _ _ _ (ok m))) in
+    {|
+    map.rep := rep;
+    map.empty := Build_rep nil eq_refl;
+    map.get m k := match List.find (fun p => key_eqb k (fst p)) (value m) with
+                   | Some (_, v) => Some v
+                   | None => None
+                   end;
+    map.put := wrapped_put;
+    map.union m1 m2 := List.fold_right (fun '(k, v) m => wrapped_put m k v) m1 (value m2)
+  |}.
+End UnorderedList.
+Arguments map : clear implicits.
