bedrock2/src/Map/SortedListString.v
@@ -1,0 +1,3 @@
+Require bedrock2.Map.SortedList bedrock2.String.
+Definition map T : bedrock2.Map.map String.string T :=
+  SortedList.map (SortedList.parameters.Build_parameters _ T String.eqb String.ltb).
