bedrock2/src/Map/SortedListString_test.v
@@ -1,0 +1,16 @@
+Require Import bedrock2.Map.
+Require bedrock2.Map.SortedListString.
+Local Existing Instance bedrock2.Map.SortedListString.map.
+Local Open Scope string_scope. Local Open Scope list_scope.
+
+Local Instance StringMapSortedList T : map.map String.string T :=
+  SortedList.map (SortedList.parameters.Build_parameters _ T String.eqb String.ltb).
+
+Import SortedList List.ListNotations.
+Goal False.
+  assert (value (map.put (map.put (map.put map.empty "a" 6) "z" 0) "c" 9) = [("a", 6); ("c", 9); ("z", 0)]%list) by exact eq_refl.
+  assert ((map.get (map.put (map.put (map.put map.empty "a" 6) "z" 0) "c" 9) "c") = Some 9) by exact eq_refl.
+  assert ((map.get (map.put (map.put (map.put map.empty "a" 6) "z" 0) "c" 9) "z") = Some 0) by exact eq_refl.
+  assert ((map.get (map.put (map.put (map.put map.empty "a" 6) "z" 0) "c" 9) "x") = None) by exact eq_refl.
+  assert (map.union (map.put (map.put map.empty "z" 7) "0" 0) (map.put (map.put (map.put map.empty "a" 6) "z" 0) "c" 9) = (map.put (map.put (map.put (map.put map.empty "a" 6) "z" 0) "c" 9) "0" 0)) by exact eq_refl.
+Abort.
